using generated ot functions

modules/clide-collaboration/src/main/isabelle/clide/collaboration/SimpleOperation.thy
@@ -1,91 +1,57 @@
 (* Formalisation of Operational Transformation *)
 (* author: Martin Ring, DFKI Bremen *) (*<*) 
 
-theory SimpleOperation
+theory Operation
 imports Main List Option Set
 begin (*>*)
 
 section {* Actions, Operations and Documents *}
 
-text {* A @{term document} is a list of elements. *}
+subsection{* Basic Types *}
+
+text {* 
+ A @{term document} is a list of arbitrary elements.
+ *}
 
 type_synonym 'char document = "'char list"
 
-text {* An @{term action} can either alter the document at the current position, move the virtual 
-        cursor on the document forward or both. *}
+text {* 
+  An operation is a sequence of elementary actions. 
+  We can think of actions as moving through a document, processing each element of the
+  document in turn to produce some output. The actions can be:
+  \begin{itemize}
+      \item @{term Retain} copies the current element to the output document;
+      \item @{term "Insert c"} inserts element @{term c} into the output document;
+      \item @{term Delete} removes the current element 
+        (i.e. does not copy it to the output document).
+   \end{itemize}
+*}
 
 datatype 'char action = Retain | Insert 'char | Delete
-
-text {* An @{term operation} is a list of actions. *}
-
 type_synonym 'char operation = "'char action list"
 
-text {* There are three types of actions of which an operation is composed:
-        @{term Retain}, @{term "Insert c"} and @{term Delete}. An operation is
-        a list of actions.
 
-        \begin{itemize}
-          \item @{term Retain} moves the cursor to the next position
-          \item @{term "Insert c"} inserts element @{term c} at the position of the cursor and moves 
-                                 the cursor behind that elment
-          \item @{term Delete} removes the element at the current position
-        \end{itemize} *}
- 
-subsection {* In- and Output Lengths of Operations *}
+subsection {* The Application Function *}
 
-text {* An operation has an input length and an output length:
+text {* 
+  The @{term applyOp} function is partial, and only defined for documents of appropriate input length.
+  *}
 
-        \begin{itemize}
-          \item The input length is the length of a document on which the operation can
-                be applied.
-          \item The output length is the length of the result of the application on a
-                document on which the operation is defined.
-        \end{itemize} *}
-
-fun inputLength :: "'char operation \<Rightarrow> nat" where
-  "inputLength [] = 0"
-| "inputLength (Retain#as) = Suc (inputLength as)"
-| "inputLength (Delete#as) = Suc (inputLength as)"
-| "inputLength (Insert _#as)  = inputLength as"
-
-text {* if an operation @{term a} has input lenght 0, a must be empty or is consists only of insert 
-        actions *}
-
-lemma emptyInputInsert [rule_format]: "inputLength a = 0 \<longrightarrow> a = [] \<or> (\<exists>as c. a = Insert c#as)"
-  by (induct_tac a rule: inputLength.induct, auto)  
-
-fun outputLength :: "'char operation \<Rightarrow> nat" where
-  "outputLength [] = 0"
-| "outputLength (Retain#as)   = Suc (outputLength as)"
-| "outputLength (Insert _#as) = Suc (outputLength as)"
-| "outputLength (Delete#as)   = outputLength as"
-
-text {* if an operation @{term a} has output lenght 0, a must be empty or is consists only of delete 
-        actions *}
-
-lemma emptyOutputDelete [rule_format]: "outputLength a = 0 \<longrightarrow> a = [] \<or> (\<exists>as. a = Delete#as)"
-  by (induct_tac a rule: outputLength.induct, auto)
-
-text {* if an operation @{term a} has output and input lenght of 0, the operation must be empty *}
-
-lemma emptyInOutOp [rule_format]: "inputLength a = 0 \<and> outputLength a = 0 \<longrightarrow> a = []"
-  by (induct_tac a rule: inputLength.induct, auto)
-
-subsection {* Application function *}
-
-text {* The @{term applyOp} function applies an operation @{term a} to document @{term d} and yields 
-        either @{term None} if the input length of @{term a} does not match the length of @{term d} 
-        or @{term "Some d'"} where @{term d'} is the result of a valid application *}
-
-fun applyOp :: "'char operation \<Rightarrow> 'char document \<Rightarrow> 'char document"
+fun applyOp :: "'char operation \<Rightarrow> 'char document \<Rightarrow> 'char document option"
 where
-  "applyOp ([])            ([])        = []"
-| "applyOp (Retain#next)   (head#tail) = head#(applyOp next tail)"
-| "applyOp (Insert c#next) (d)         = c#(applyOp next d)"
-| "applyOp (Delete#next)   (_#tail)    = applyOp next tail"
+  "applyOp [] []                       = Some []"
+| "applyOp (Retain# as) (b# bs) = Option.map (\<lambda>ds. b# ds) (applyOp as bs)"
+| "applyOp (Insert c# as) bs       = Option.map (\<lambda>ds. c# ds) (applyOp as bs)"
+| "applyOp (Delete# as) (_# bs)  = applyOp as bs"
+| "applyOp _  _                        = None"
            
-text {* We also define an inductive set, describing the relation of all valid pairs of operations and 
-        documents and their resulting output document .*}
+text {* 
+  Here is an example of an operation, and how it is being applied:
+  \[ @{lemma "applyOp [Retain, Delete, Insert b, Retain] [a, x, c] = Some [a, b, c]" by simp} \]
+
+  We now define the graph of the function @{term applyOp} as an inductive set; this makes
+  inductive reasoning about @{term applyOp} easier.
+  *}
 
 inductive_set application :: "(('char operation \<times> 'char document) \<times> 'char document) set" where
   empty[intro!]:  "(([],[]),[]) \<in> application"
@@ -93,29 +59,89 @@ inductive_set application :: "(('char operation \<times> 'char document) \<times
 | delete[intro!]: "((a,d),d') \<in> application \<Longrightarrow> ((Delete#a,c#d),d')     \<in> application"
 | insert[intro!]: "((a,d),d') \<in> application \<Longrightarrow> (((Insert c)#a,d),c#d') \<in> application"
 
-text {* We need to show the equality of the inductively defined set @{term application} and the partial
-        function @{term applyOp} in order to use the inductive set for further correctness proofs
-        involving @{term applyOp} *}
+text {* 
+  We need to show the equality of the inductively defined set @{term application} and the partial
+  function @{term applyOp} in order to use the inductive set for further proofs. We prove the 
+  required eqivalence in both directions separately. 
+  *}
 
-lemma applyOpSet: "((a,d),d') \<in> application \<Longrightarrow> applyOp a d = d'"
+lemma applyOpSet1 [rule_format]: 
+  "\<forall>d'. applyOp a d = Some d' \<longrightarrow> ((a,d),d') \<in> application"
+  by (rule applyOp.induct, auto)
+
+lemma applyOpSet2: 
+  "((a,d),d') \<in> application \<Longrightarrow> applyOp a d = Some d'"
   by (erule application.induct, auto)
 
-text {* this also implicitly proves that the relation @{term application} is deterministic *}
-
-subsection {* Valid Operations *}
-
-text {* iff an operation @{term a} is empty it can only be applied to the empty document and the
-        result is also the empty document *}
-
-lemma emptyInput: "(([],d),d') \<in> application \<longleftrightarrow> d = [] \<and> d' = []"  
-  apply (auto)
-  by (metis application.cases list.distinct(1))+
-
-lemma emptyDocInsert: "(\<exists>d'. (((a#as),[]),d') \<in> application) \<longrightarrow> (\<exists>c. a = Insert c)"
-  apply (case_tac a, auto)
-  apply (metis action.distinct(1) application.simps list.distinct(1) list.inject)  
-  by (metis action.distinct(5) application.cases list.distinct(1) list.inject)
+lemma applyOpSet: "applyOp a d = Some d' \<longleftrightarrow> ((a,d),d') \<in> application"
+  by (force intro: applyOpSet1 applyOpSet2)
   
+subsection {* Input and Output Lengths *}
+
+text{*
+  Operations are partial, and can only be applied to documents of a specific length, 
+  called the inputLength. The output length is the length of the result
+  of the application on a document on which the operation is defined.
+  
+  The input length is the number of @{term Retain} and @{term Delete} actions, whereas
+  the output length is the number of @{term Retain} and @{term Insert} actions.
+*}
+
+fun inputLength :: "'char operation \<Rightarrow> nat" where
+  "inputLength [] = 0"
+| "inputLength (Retain# as) = Suc (inputLength as)"
+| "inputLength (Delete# as) = Suc (inputLength as)"
+| "inputLength (Insert _# as)  = inputLength as"
+
+fun outputLength :: "'char operation \<Rightarrow> nat" where
+  "outputLength [] = 0"
+| "outputLength (Retain# as)   = Suc (outputLength as)"
+| "outputLength (Insert _# as) = Suc (outputLength as)"
+| "outputLength (Delete# as)   = outputLength as"
+
+text {* 
+ Some lemmas to characterise operations by their length. If an operation @{term b} has input lenght 0, 
+ @{term b} must contain only insert actions (or be empty); if an operation @{term b} has output
+ length 0, @{term b} must contain only delete actions (or be empty); and if both input and 
+ output length are 0, then @{term a} must be empty.
+ *}
+
+lemma emptyInputLength [rule_format]: "inputLength b = 0 \<longrightarrow> (\<forall> a \<in> set b. \<exists>c. a = Insert c)"
+  by (induct_tac b rule: inputLength.induct,  force+)
+  
+lemma emptyOutputLength [rule_format]: "outputLength b = 0 \<longrightarrow> (\<forall> a \<in> set b. a = Delete)"
+  by (induct_tac b rule: outputLength.induct, force+)
+
+lemma emptyInOutLength [rule_format]: "inputLength a = 0 \<and> outputLength a = 0 \<longrightarrow> a = []"
+  by (induct_tac a rule: inputLength.induct, auto)
+
+text{*
+ The following two lemmas show that @{term validInputLength} and @{term outputLength} really do
+ as advertised. 
+ *}
+
+lemma validInputLength: "(\<exists>d'. applyOp a d = Some d') \<longleftrightarrow> (inputLength a = length d)"
+  by (induct_tac a d rule: applyOp.induct, auto)
+  
+lemma validOutputLength: "(applyOp a d = Some d') \<Longrightarrow> (outputLength a= length d')"
+  apply (simp add: applyOpSet)
+  apply (erule application.induct, auto)
+  done
+
+subsection{* Semantics of Actions *}
+
+text {* 
+  A preliminary: an operation is empty iff it can only be applied to the empty document 
+  and the result is also the empty document. The empty operation is, of course, the empty list. *}
+
+lemma emptyInput: "applyOp [] d = Some d' \<longleftrightarrow> d = [] \<and> d' = []"
+  by (induct_tac d, auto)
+
+text{*
+  The following three lemmas characterise the semantics of the basic actions in terms of
+  the @{term application} set; e.g. the first one says that @{term Retain} copies the 
+  character @{term c} from the input document to the output document.
+  *}
 lemma remRetain: "(((Retain#as,d),d') \<in> application) =
                    (\<exists>c cs cs'. d = c#cs \<and> d'=c#cs' \<and> ((as,cs),cs') \<in> application)"
   apply (auto)
@@ -130,124 +156,91 @@ lemma remDelete: "(((Delete # list, d),d') \<in> application) =
                   (\<exists>c cs. d = c#cs \<and> ((list,cs),d') \<in> application)"  
   apply (auto)
   by (smt action.distinct(3) application.cases inputLength.simps(3) inputLength.simps(4) list.distinct(1) list.inject)
-
-text {* every document can be produced by the application of an operation to a document *}
-
-lemma applicationRange: "\<exists>a d. ((a,d),d') \<in> application"
-  by (induct_tac d', auto)
-
-subsection {* In- and Output Lenghts of Valid Operations *}
-
-text {* All pairs of operations and documents are contained in the domain of the application
-        iff the inputLength of the operation matches the length of the document *}
-
-lemma applicationDomain: "(\<exists>d'. ((a,d),d') \<in> application) \<longleftrightarrow> (inputLength a = length d)"
-  sorry
   
-text {* if an operation @{term a} is a valid operation on any document @{term d} the length of the 
-        resulting document @{term d'} is equal to the output lenght of @{term a} *}
+section{* Composition *}
 
-lemma validOutputLength: "((a,d),d') \<in> application \<Longrightarrow> outputLength a = length d'"
-  by (erule application.induct, auto)
+subsection{* The Function @{term addDeleteOp} *}
 
-subsection {* Normalization *}
+text{*
+  The function @{term addDeleteOp} is an optimisation. It starts from the observation that 
+  @{term Delete} and @{term "Insert c"} actions commute, i.e. we can exchange them and still get
+  the same operation:
+  \[ @{lemma "applyOp [Delete, Insert c] [x] = applyOp [Insert c, Delete] [x]" by simp } \]
+  Hence, it makes sense to sort sequences of @{term Delete} and @{term Insert} actions in such
+  a way that we get sequences contiguous @{term Delete} and @{term Insert} actions; we can then
+  compress into one parameterised delelte action, or an insert action which takes a string as 
+  argument.The @{term addDeleteOp} fuction adds a delete action, but commutes it as far back 
+  into the argument as possible.
+  *}  
 
 fun addDeleteOp :: "'char operation \<Rightarrow> 'char operation"
 where
-  "addDeleteOp (Insert c#next) = (Insert c)#(addDeleteOp next)"
-| "addDeleteOp as = Delete#as"
+  "addDeleteOp (Insert c# next) = Insert c# addDeleteOp next"
+| "addDeleteOp as = Delete# as"
 
-lemma addDeleteOpValid11: "((a,d),d') \<in> application \<Longrightarrow> \<forall>c. ((addDeleteOp a,c#d),d') \<in> application"
+
+text{* 
+  After two auxiliary lemmas  we will show that @{term addDeleteOp} really adds a delete action,
+  in the sense that if we apply it then it removes the first element of the document.
+  *}
+ 
+lemma addDeleteOpValid11[rule_format]: "((a,d),d') \<in> application \<Longrightarrow> \<forall>c. ((addDeleteOp a,c#d),d') \<in> application"
   by (rule application.induct, auto)
 
 lemma addDeleteOpValid1: "((Delete#as,d),d') \<in> application \<Longrightarrow> ((addDeleteOp as,d),d') \<in> application"
   by (smt action.distinct(3) action.distinct(5) addDeleteOpValid11 application.cases list.distinct(1) list.inject)
 
-lemma addDeleteOpValid: "((a,d),d') \<in> application \<Longrightarrow> \<forall>c. ((addDeleteOp a,c#d),d') \<in> application"
-  by (simp add: addDeleteOpValid11)
-
-lemma addDeleteOutputLenght[simp]: "outputLength (addDeleteOp as) = outputLength as"
+lemma addDeleteOpValid: "applyOp (addDeleteOp a) (c#d) = applyOp a d"
   by (rule addDeleteOp.induct, auto)
 
-text {* The @{term normalize} function sorts all sequences within an operation that do not contain
-        {@term Retain} actions, such that all @{term Insert} actions occur before the @{term Delete}
-        actions *}
+text{* 
+  As can be expected, @{term addDeleteOp} does not change the @{term outputLength}. 
+  This lemma is actually not needed in the following.
+  *}
+lemma addDeleteOutputLength: "outputLength (addDeleteOp as) = outputLength as"
+  by (rule addDeleteOp.induct, auto)
 
-fun normalize :: "'char operation \<Rightarrow> 'char operation" where
-  "normalize [] = []"
-| "normalize (Retain#a) = Retain#(normalize a)"
-| "normalize (Insert c#a) = Insert c#(normalize a)"
-| "normalize (Delete#a) = addDeleteOp (normalize a)"
+subsection {* Composition of Operations *}
 
-value "normalize [Delete, Insert a, Delete, Insert b, Retain, Insert c]"
-
-text {* For @{term normalize} to be useful it must not change the effect of an operation:
-
-        if an operation $a$ can be applied to a document $d$ yielding the resulting document $d'$,
-        the normalized operation $a$ can also be applied to the document $d$ yielding the same 
-        result *}
-
-lemma normalizeValid: "((a,d),d') \<in> application \<Longrightarrow> ((normalize a,d),d') \<in> application"
-  apply (erule application.induct)
-  apply (auto intro: addDeleteOpValid1)
-  done
-
-text {* if @{term addDeleteOp} is called on a normalized operation the resulting operation is also
-        normalized *}
-
-lemma normalizeAddDeleteOp[rule_format]: "normalize a = a \<longrightarrow> addDeleteOp a = normalize (addDeleteOp a)"
-  apply (induct_tac a)
-  apply (simp)
-  apply (case_tac a, simp_all)
-  done
-
-lemma normalizeAddDeleteOp2[rule_format]: "normalize a = a \<longrightarrow> addDeleteOp a = normalize (Delete#a)"
-  apply (induct_tac a)
-  apply (simp)
-  apply (case_tac a, simp_all)
-  done
-
-section {* Composition of Operations *}
-
-text {* The @{term compose} function composes two operations @{term a} and @{term b}, in such a way
-        that the composed operation @{term ab} has the same effect upon application as operations
-        @{term a} and @{term b} executed sequentially. *}
+text {* 
+  The @{term compose} function composes two operations @{term a} and @{term b}, in such a way
+  that the composed operation @{term ab} has the same effect upon application as operations
+  @{term a} and @{term b} executed sequentially.  
+*}
 
 fun compose :: "'char operation \<Rightarrow> 'char operation \<Rightarrow> 'char operation option"
 where
-  "compose [] []                        = Some []"
-| "compose (Delete#as)    (bs)          = Option.map addDeleteOp (compose as bs)"
-| "compose (as)           (Insert c#bs) = Option.map (Cons (Insert c)) (compose as bs)"
-| "compose (Retain#as)    (Retain#bs)   = Option.map (Cons Retain) (compose as bs)"
-| "compose (Retain#as)    (Delete#bs)   = Option.map addDeleteOp (compose as bs)"
-| "compose (Insert(c)#as) (Retain#bs)   = Option.map (Cons (Insert c)) (compose as bs)"
-| "compose (Insert(_)#as) (Delete#bs)   = compose as bs"
-| "compose _              _             = None"
-
-subsection {* Normalized Output *}
-
-text {* the result of @{term compose} is always normalized *}
-
-lemma composeNormalized[rule_format]: "\<forall>ab. compose a b = Some ab \<longrightarrow> ab = normalize ab"
-  apply (rule compose.induct, auto)  
-  apply (rule normalizeAddDeleteOp, simp)+
-  done
-
-subsection {* Inductive Set *}
-
-text {* Again we define an inductive set describing the composition relation. *}
+  "compose [] []                              = Some []"
+| "compose (Delete# as) bs               = Option.map addDeleteOp (compose as bs)"
+| "compose as (Insert c# bs)             = Option.map (Cons (Insert c)) (compose as bs)"
+| "compose (Retain# as) (Retain# bs) = Option.map (Cons Retain) (compose as bs)"
+| "compose (Retain# as) (Delete# bs)  = Option.map addDeleteOp (compose as bs)"
+| "compose (Insert c# as) (Retain# bs) = Option.map (Cons (Insert c)) (compose as bs)"
+| "compose (Insert _# as) (Delete# bs) = compose as bs"
+| "compose _ _                                = None"
+ 
+text{* 
+  Here is an example of how compose works:
+  \[ @{lemma "compose [Retain, Delete, Insert b, Retain] [Retain, Retain, Insert c, Delete] 
+               = Some [Retain, Insert b, Insert c, Delete, Delete]" by simp } \]
+  Note how the @{term Insert} and @{term Delete} actions are grouped together.
+  
+  Following the approach from above, we define the graph of @{term compose} as an inductive set.
+  *}
 
 inductive_set composition :: "(('char operation \<times> 'char operation) \<times> 'char operation) set" where
   empty[intro!]:  "(([],[]),[]) \<in> composition"
-| [intro!]: "((a,b),ab) \<in> composition \<Longrightarrow> ((Delete#a,b),addDeleteOp ab) \<in> composition"
-| [intro!]: "((a,b),ab) \<in> composition \<Longrightarrow> ((a,Insert c#b),Insert c#ab) \<in> composition"
-| [intro!]: "((a,b),ab) \<in> composition \<Longrightarrow> ((Retain#a,Retain#b),Retain#ab) \<in> composition"
-| [intro!]: "((a,b),ab) \<in> composition \<Longrightarrow> ((Retain#a,Delete#b),addDeleteOp ab) \<in> composition"
-| [intro!]: "((a,b),ab) \<in> composition \<Longrightarrow> ((Insert c#a,Retain#b),Insert c#ab) \<in> composition"
-| [intro!]: "((a,b),ab) \<in> composition \<Longrightarrow> ((Insert _#a,Delete#b),ab) \<in> composition"
+| [intro!]: "((a,b),ab) \<in> composition \<Longrightarrow> ((Delete# a,b), addDeleteOp ab) \<in> composition"
+| [intro!]: "((a,b),ab) \<in> composition \<Longrightarrow> ((a, Insert c#b), Insert c# ab) \<in> composition"
+| [intro!]: "((a,b),ab) \<in> composition \<Longrightarrow> ((Retain# a, Retain#b), Retain# ab) \<in> composition"
+| [intro!]: "((a,b),ab) \<in> composition \<Longrightarrow> ((Retain# a, Delete#b), addDeleteOp ab) \<in> composition"
+| [intro!]: "((a,b),ab) \<in> composition \<Longrightarrow> ((Insert c# a, Retain# b),Insert c# ab) \<in> composition"
+| [intro!]: "((a,b),ab) \<in> composition \<Longrightarrow> ((Insert _# a, Delete# b),ab) \<in> composition"
 
-text {* And again we have to prove equivalence of the inductively defined relation and the 
-        recursive function: *}
+text {* 
+  And again we prove that this set is graph of @{term compose}.
+  We first need three lemmas, then the main lemma.
+  *}
 
 lemma composeSet11 [rule_format]: 
   "\<forall>ab c. compose a b = Some ab \<longrightarrow> compose a (Insert c # b) = Some (Insert c # ab)"
@@ -261,13 +254,15 @@ lemma composeSet2 [rule_format]: "\<forall>ab. compose a b = Some ab \<longright
   apply (auto)
   done
 
-lemma composeSet: "((a,b),ab) \<in> composition \<longleftrightarrow> compose a b = Some (ab)"
+lemma composeSet: "((a,b), ab) \<in> composition \<longleftrightarrow> compose a b = Some ab"
   by (auto intro: composeSet1 composeSet2)
 
-subsection {* Domain *}
+subsection {* Composable Operations. *}
 
-text {* The operations @{term a} and @{term b} can be composed iff the output length of @{term a} 
-        matches the input length of @{term b} *}
+text {* 
+  The operations @{term a} and @{term b} can be composed iff the output length of @{term a} 
+  is the input length of @{term b}. We need three lemmas before the main result. 
+  *}
 
 lemma composeDomain1 [rule_format]: "(\<exists>ab. compose a b = Some ab) \<longrightarrow> outputLength a = inputLength b"
   by (rule compose.induct, auto)
@@ -281,49 +276,61 @@ lemma composeDomain2: "outputLength a = inputLength b \<Longrightarrow> (\<exist
 
 lemma composeDomain: "(\<exists>ab. compose a b = Some ab) \<longleftrightarrow> outputLength a = inputLength b"
   by (auto intro: composeDomain1 composeDomain2)
+    
+subsection{* Correctness of the Composition *}
 
-subsection {* Range *}
-
-text {* Every operation $ab$ can be produced in its normalized form by composition of two 
-        operations  *}
-
-lemma compositionRange: "(normalize ab) \<in> Range composition"
-  by (rule normalize.induct, auto)
-
-subsection {* Invariant of the composition *}
-
-text {* Finally we show that the @{term compose} function does actually compose operations *}
+text {* 
+  Finally, we show that the @{term compose} function does actually compose operations, in the 
+  sense that applying the composed operation is the same as applying the two arguments consecutively.
+  We first show this using the graph @{term composition}, then transfer this to the function using the 
+  conversion theorems @{text applyOpSet} and @{text composeSet}.
+  *}
 
 lemma compositionInv [rule_format]: "((a,b),ab) \<in> composition \<Longrightarrow> \<forall>d d' d''. ((a,d),d') \<in> application \<longrightarrow> ((b,d'),d'') \<in> application \<longrightarrow> ((ab,d),d'') \<in> application"
   apply (erule composition.induct)
-  by (auto simp add: emptyInput addDeleteOpValid11 remDelete remInsert remRetain)  
+  apply (auto simp add: emptyInput addDeleteOpValid11 remDelete remInsert remRetain)
+  by (metis applyOpSet emptyInput)
   
-section {* Operation Transformation *}
+theorem composeCorrect: 
+  "\<lbrakk> compose a b = Some ab; applyOp a d = Some d'; applyOp b d' = Some d'' \<rbrakk> 
+   \<Longrightarrow> applyOp ab d = Some d''"
+  by (simp add: composeSet applyOpSet compositionInv)
 
-text {* The transformation function is the basis of operational transformation. For a pair of 
-        operations @{term "(a,b)"} it computes an output pair of transformed operations 
-        @{term "(a',b')"}. The convergence property @{term "compose a b' = compose b a'"} enables
-        the OT system to execute operations in different order at different sites while the 
-        documents do not diverge *}
+section{* Transforming Operations *}
+
+text {* 
+  The transformation function is the basis of operational transformation. For a pair of 
+  operations @{term "(a,b)"} it computes an output pair of transformed operations 
+  @{term "(a',b')"}, such that @{term "compose a b' = compose b a'"}; this is the 
+  main correctness property of operational transformation.
+  *}
 
 fun transform :: "'char operation \<Rightarrow> 'char operation \<Rightarrow> ('char operation \<times> 'char operation) option"
 where
-  "transform []             []             = Some ([],[])"
-| "transform (Insert(c)#as) b              = Option.map (\<lambda>(at,bt). (Insert(c)#at,Retain#bt)) (transform as b)"
-| "transform a              (Insert(c)#bs) = Option.map (\<lambda>(at,bt). (Retain#at,Insert(c)#bt)) (transform a bs)"
-| "transform (Retain#as)    (Retain#bs)    = Option.map (\<lambda>(at,bt). (Retain#at,Retain#bt)) (transform as bs)"
-| "transform (Delete#as)    (Delete#bs)    = transform as bs"
-| "transform (Retain#as)    (Delete#bs)    = Option.map (\<lambda>(at,bt). (at,Delete#bt)) (transform as bs)"
-| "transform (Delete#as)    (Retain#bs)    = Option.map (\<lambda>(at,bt). (Delete#at,bt)) (transform as bs)"
-| "transform _              _              = None"
+  "transform [] []                 = Some ([], [])"
+| "transform (Insert c#as) bs  = 
+              Option.map (\<lambda>(at, bt). (Insert c# at, Retain# bt)) (transform as bs)"
+| "transform as (Insert c# bs) = 
+              Option.map (\<lambda>(at, bt). (Retain# at, Insert c# bt)) (transform as bs)"
+| "transform (Retain# as) (Retain# bs) = 
+              Option.map (\<lambda>(at, bt). (Retain# at, Retain# bt)) (transform as bs)"
+| "transform (Delete# as) (Delete# bs) = transform as bs"
+| "transform (Retain# as) (Delete# bs) = 
+              Option.map (\<lambda>(at, bt). (at, Delete# bt)) (transform as bs)"
+| "transform (Delete# as) (Retain# bs) = 
+              Option.map (\<lambda>(at, bt). (Delete# at, bt)) (transform as bs)"
+| "transform _ _                           = None"
 
-text {* the transformation of two operations yields a result iff they have an equal input length *}
+text {* 
+  The transformation of two operations yields a result iff they have an equal input length.
+  *}
 
 lemma transformDomain: "(\<exists>ab. transform a b = Some ab) \<longleftrightarrow> inputLength a = inputLength b"
   by (induct_tac a b rule: transform.induct, auto)  
 
-text {* Yet again we define an inductive set to describe the transform relation. Again we omit all
-        applications of @{term addDeleteOp} and replace them by @{term Delete} *}
+text {* 
+  Again, we define its graph inductively.
+  *}
 
 inductive_set transformation :: "(('c operation \<times> 'c operation) \<times> ('c operation \<times> 'c operation)) set" where
   empty[intro!]: "(([],[]),([],[])) \<in> transformation"
@@ -336,25 +343,172 @@ inductive_set transformation :: "(('c operation \<times> 'c operation) \<times> 
 | [intro!]: "((a,b),(a',b')) \<in> transformation \<Longrightarrow> ((Retain#a,Delete#b),(a',Delete#b')) \<in> transformation"
 | [intro!]: "((a,b),(a',b')) \<in> transformation \<Longrightarrow> ((Delete#a,Retain#b),(Delete#a',b')) \<in> transformation"
 
-text {* we need to show, that the above relation is a superset of the @{term transform} function *}
+text{*
+  Here, it is enough to show that this set is a superset of the function graph.
+  *}
 
 lemma transformSubset[rule_format]: "\<forall>a' b'. transform a b = Some (a',b') \<longrightarrow> ((a,b),(a',b')) \<in> transformation"
   by (rule transform.induct, auto)  
 
-text {* And finally we show the convergence property for the set ... *}
+text {* 
+  We can now show the main correctness property, first for the set @{term transformation}. 
+  *}
 
-lemma transformationConvergence: "((a,b),(a',b')) \<in> transformation \<Longrightarrow>
-                                   (\<exists>ab. ((a,b'),ab) \<in> composition \<and> ((b,a'),ab) \<in> composition)"
-  by (erule transformation.induct, auto)
+lemma transformationConvergence: "((a,b), (a',b')) \<in> transformation \<Longrightarrow>
+                                   (\<exists>ab. ((a,b'), ab) \<in> composition \<and> ((b,a'), ab) \<in> composition)"
+  by (erule transformation.induct, auto)  
 
-text {* ... and for the @{term transform} function *}
+text {* 
+  We now show the correctness of the @{term transform} function. Because the equality involving
+  @{term transform} occurs only in the precondition, we only need that @{term transformation} is a 
+  superset of the function graph to reduce that precondition to the one of @{text transformationConvergence}.
+  *}
 
-lemma tp1: "transform a b = Some (a',b') \<Longrightarrow> compose a b' \<noteq> None \<and> compose a b' = compose b a'"  
+theorem transformCorrect: "transform a b = Some (a',b')
+  \<Longrightarrow> compose a b' \<noteq> None \<and> compose a b' = compose b a'"  
   apply (drule transformSubset)
   apply (drule transformationConvergence)
   by (auto simp add: composeSet)  
 
-(*export_code applyOp addDeleteOp compose transform in Scala
-  module_name Operation*)
+text{*  
+  This concludes the main development. 
+  *}
+  
+section{* Normalization *}
+
+text {*
+ Normalisation is what occurs during composition. We say an operation is normalised if 
+ there is no @{term Delete} operation followed by an @{term Insert}. (We could do this the other
+ way around, but have to pick on one order.)  
+ *}
+ 
+fun normalized :: "'char operation \<Rightarrow> bool"
+where
+  "normalized [] = True"
+| "normalized (Delete# (Insert _# _))= False"
+| "normalized (_ # as) = normalized as"
+
+text{*
+ The @{term normalize} function sorts all those subsequences not containing @{term Retain} actions,
+ such that all @{term Insert} actions occur before the @{term Delete} actions.
+ *}
+
+fun normalize :: "'char operation \<Rightarrow> 'char operation" where
+  "normalize [] = []"
+| "normalize (Retain#a) = Retain#(normalize a)"
+| "normalize (Insert c#a) = Insert c#(normalize a)"
+| "normalize (Delete#a) = addDeleteOp (normalize a)"
+
+text{*
+  Here is an example of how normalize works:
+  \[ @{lemma "normalize [Delete, Insert a, Delete, Insert b, Retain, Insert c] = [Insert a, Insert b, Delete, Delete, Retain, Insert c]" by simp} \]
+
+  To show correctness of @{term normalizes}, we first need lemma that @{term addDeletOp} preserves
+  normalisation. 
+  *}
+
+lemma addDeleteOpNormalized[rule_format]: "normalized a \<longrightarrow> normalized (addDeleteOp a)"
+  by (induct a rule: addDeleteOp.induct, simp_all)
+
+lemma normalizes: "normalized (normalize a)"
+  by (induct a rule: normalize.induct, simp_all add: addDeleteOpNormalized)
+
+text{*
+  We also show that normalized operations are fixpoints of the @{term normalize} function,
+  or in more elementary terms, normalizing once is enough.
+  *}
+  
+lemma normalized_fix: "normalized a \<longleftrightarrow> (normalize a= a)"
+  apply (rule iffI)
+  apply (induct a rule: normalize.induct)
+  apply (simp_all)
+  apply (case_tac "a", simp)
+  apply (case_tac "aa", simp_all)
+  apply (rule subst [where P="normalized"]) --{* Strange, we have to do this by hand. *}
+  apply (assumption, rule normalizes)
+  done
+
+text {* 
+ @{term normalize} should not change the effect of an operation:
+ if an operation $a$ can be applied to a document $d$ yielding the resulting document $d'$,
+ the normalized operation $a$ can also be applied to the document $d$ yielding the same 
+ result.
+*}
+
+lemma normalizeValid1: "((a,d),d') \<in> application \<Longrightarrow> ((normalize a,d),d') \<in> application"
+  apply (erule application.induct)
+  apply (auto intro: addDeleteOpValid1)
+  done
+
+lemma normalizeValid: "applyOp a d = Some d' \<Longrightarrow> applyOp(normalize a) d= Some d'"
+  apply (fast intro: applyOpSet2 applyOpSet1 normalizeValid1)
+  done
+
+
+text{* The result of @{term compose} is always normalized. *}
+
+lemma composeNormalized[rule_format]: "\<forall>ab. compose a b = Some ab \<longrightarrow> normalized ab"
+  by (rule compose.induct, auto intro:  addDeleteOpNormalized)
+
+section{* Identities *}
+
+text{*
+  The identity operation consists of only @{term Retain} actions. In fact, the identity
+  operation is parameterised over the length of the argument, so there is one identity
+  for each document length.
+  *}
+
+fun ident :: "nat=> 'char operation"
+where
+  "ident n = replicate n Retain"
+
+text{*
+  @{term ident} has exactly the input and output lengths that we expect.
+  *}
+
+lemma identInputLength: "inputLength (ident n)= n"
+ by (induct n, auto)
+
+lemma identOutputLength: "outputLength (ident n)= n"
+ by (induct n, auto)
+
+text{*
+  Moreover, @{term ident} behaves as a left and right unit to the composition, but 
+  note that it is only equal up to normalisation, as composition normalises its result.
+  *}
+ 
+lemma composeIdL: "compose (ident (inputLength b)) b = Some (normalize b)"
+  apply (induct_tac b, simp)
+  apply (case_tac "inputLength list")
+  apply (case_tac a, simp_all)
+  by (case_tac a, simp_all)
+
+lemma composeIdR: "compose b (ident (outputLength b))= Some (normalize b)"
+  apply (induct_tac b, simp)
+  apply (case_tac "inputLength list")
+  apply (case_tac a, simp_all)
+  by (case_tac a, simp_all)
+
+text{*
+  Transforming against @{term ident} does not change the operation (it does not 
+  even normalize), and @{term ident} transformed gives the identity again.
+  *}
+  
+lemma transformIdL: 
+  "transform (ident (inputLength b)) b = Some (ident (outputLength b), b)"
+  apply (induct_tac b, simp)
+  apply (case_tac "inputLength list")
+  apply (case_tac a, simp_all)
+  by (case_tac a, simp_all)
+
+lemma transformIdR: 
+  "transform b (ident (inputLength b))= Some (b, ident (outputLength b))"
+  apply (induct_tac b, simp)
+  apply (case_tac "inputLength list")
+  apply (case_tac a, simp_all)
+  by (case_tac a, simp_all)
+  
+export_code applyOp compose transform in Scala
+  module_name Operation
 
 end
